<?xml version="1.0" encoding="UTF-8"?>

<section xml:id="sec_fourth-dynamics" xmlns:xi="http://www.w3.org/2001/XInclude">
  <title>Dynamics</title>
  
   <introduction>
    <p>
      Dynamics in physics explains the causes of motion. 
      In dynamics <m>v\neq 0, \quad a\neq 0,</m> and <m>F\neq 0</m>.
      From Newton's Second Law: 
      <me>
        \sum \vec{F}  =  m \vec{a}
      </me>
      or, equivalently
      <me>
        \sum F_{x}  =  m a_{x} 
      </me>
      (x-component of <m>\vec{F}</m>), and
      <me>
        \sum F_{y}  =  m a_{y}	
      </me>
      (y-component <m>\vec{F}</m>)
        For gravitational force or weight, <m>F = mg</m>.
    </p>
   </introduction>

   <subsection xml:id="subsec-atwood_machine">
    <title>Atwood's Machine</title>
    <p>
      It is device where two masses <m>m_{1}</m> and <m>m_{2}</m> are hung at 
      both ends of a massless,  unstretchable string that runs over a frictionless 
      and massless pulley as shown in figure below. This machine is used to learn 
      the concept of dynamics in a little complex condition. In massless and frictionless 
      pulley tension on both sides of the string and the magnitude of acceleration of 
      both masses remain the same as there is no slack in the string as it moves.
    </p>
    <figure>
      <caption></caption>
      <sidebyside widths="30% 20% 20% 25%">
        <figure xml:id="Atwood1">
          <caption></caption>
          <image source="Atwood1.png"/>
      </figure>
          <figure xml:id="Atwood2">
              <caption></caption>
              <image source="Atwood2.png"/>
          </figure>
          <figure xml:id="Atwood3">
              <caption></caption>
              <image source="Atwood3.png"/>
          </figure>
          <figure xml:id="Atwood4">
            <caption></caption>
            <image source="Atwood4.png"/>
        </figure>
       </sidebyside>
  </figure>

  <p>
    From  free body diagram <xref ref="Atwood1"/>, we have -
    <men xml:id="eqn-atwood1">
      m_{0}g-T_{1} =m_{1}a \quad \Rightarrow \quad T_{1} = m_{1}g-m_{1}a  
    </men>
    From  free body diagram <xref ref="Atwood2"/>, we have -
    <men xml:id="eqn-atwood2">
      T_{1}-m_{2}g- =m_{2}a  \quad \Rightarrow \quad T_{2} = m_{2}g+m_{2}a  
    </men>
    System as a whole from figure  <xref ref="Atwood1"/>, we have - 
    <me>
      F_{net} = (m_{1}+m_{2})a
    </me>
    <men xml:id="eqn-atwood3">
      \text{or,}\quad m_{1}g-m_{2}g = (m_{1}+m_{2})a\quad  \Rightarrow \quad a=\frac{(m_{1}-m_{2})g}{(m_{1}+m_{2})}  
    </men>
  Therefore from eqn. <xref ref="eqn-atwood1"/>, we get -
  <men xml:id="eqn-atwood4">
    T_{1} =  m_{1}g-m_{1}\frac{(m_{1}-m_{2})g}{(m_{1}+m_{2})}= \frac{2m_{1}m_{2}g}{(m_{1}+m_{2})}  
  </men>
  Also from eqn.<xref ref="eqn-atwood2"/>, we get -
  <men xml:id="eqn-atwood5">
    T_{2} =  m_{2}g+m_{2}\frac{(m_{1}-m_{2})g}{(m_{1}+m_{2})}= \frac{2m_{1}m_{2}g}{(m_{1}+m_{2})}
  </men>
 Hence from eqns.<xref ref="eqn-atwood4"/> and <xref ref="eqn-atwood5"/>, 
 it is clear that <m>T_{1}=T_{2}</m> in massless and frictionless pulley. 
 We can see in rigid body dynamics that when pulley has mass and friction, 
 <m>T_{1}</m> is no longer equal to <m>T_{2}</m>. 
</p> 
<p>
Now, we can evaluate velocity of masses as 
 <me>
  a=\frac{(m_{1}-m_{2})g}{(m_{1}+m_{2})} 
 </me>
</p>
  
   </subsection>

  </section>

